feat: linear integer inequality normalization using `gcd` of coefficients (#7030)
This PR adds completes the linear integer inequality normalizer for
`grind`. The missing normalization step replaces a linear inequality of
the form `a_1*x_1 + ... + a_n*x_n + b <= 0` with `a_1/k * x_1 + ... +
a_n/k * x_n + ceil(b/k) <= 0` where `k = gcd(a_1, ..., a_n)`.
`ceil(b/k)` is implemented using the helper `cdiv b k`.

src/Init/Data/Int/Linear.lean
@@ -98,8 +98,53 @@ def PolyCnstr.denote (ctx : Context) : PolyCnstr → Prop
   | .eq p => p.denote ctx = 0
   | .le p => p.denote ctx ≤ 0
 
+def cdiv (a b : Int) : Int :=
+  -((-a)/b)
+
+def cmod (a b : Int) : Int :=
+  -((-a)%b)
+
+theorem cdiv_add_cmod (a b : Int) : b*(cdiv a b) + cmod a b = a := by
+  unfold cdiv cmod
+  have := Int.ediv_add_emod (-a) b
+  have := congrArg (Neg.neg) this
+  simp at this
+  conv => rhs; rw[← this]
+  rw [Int.neg_add, ←Int.neg_mul, Int.neg_mul_comm]
+
+theorem cmod_gt_of_pos (a : Int) {b : Int} (h : 0 < b) : cmod a b > -b :=
+  Int.neg_lt_neg (Int.emod_lt_of_pos (-a) h)
+
+theorem cmod_nonpos (a : Int) {b : Int} (h : b ≠ 0) : cmod a b ≤ 0 := by
+  have := Int.neg_le_neg (Int.emod_nonneg (-a) h)
+  simp at this
+  assumption
+
+theorem cmod_eq_zero_iff_emod_eq_zero (a b : Int) : cmod a b = 0 ↔ a%b = 0 := by
+  unfold cmod
+  have := @Int.emod_eq_emod_iff_emod_sub_eq_zero  b b a
+  simp at this
+  simp [Int.neg_emod, ← this, Eq.comm]
+
+theorem cdiv_eq_div_of_divides {a b : Int} (h : (a/b)*b = a) : a/b = cdiv a b := by
+  have hz : a % b = 0 := by
+    have := Int.ediv_add_emod a b
+    conv at this => rhs; rw [← Int.add_zero a]
+    rw [Int.mul_comm, h] at this
+    exact Int.add_left_cancel this
+  have hcz : cmod a b = 0 := cmod_eq_zero_iff_emod_eq_zero a b |>.mpr hz
+  have : (cdiv a b)*b = a := by
+    have := cdiv_add_cmod a b
+    simp [hcz] at this
+    rw [Int.mul_comm] at this
+    assumption
+  have : (a/b)*b = (cdiv a b)*b := Eq.trans h this.symm
+  by_cases h : b = 0
+  next => simp[cdiv, h]
+  next => rw [Int.mul_eq_mul_right_iff h] at this; assumption
+
 def Poly.div (k : Int) : Poly → Poly
-  | .num k' => .num (k'/k)
+  | .num k' => .num (cdiv k' k)
   | .add k' x p => .add (k'/k) x (div k p)
 
 def Poly.divAll (k : Int) : Poly → Bool
@@ -119,8 +164,14 @@ def PolyCnstr.norm : PolyCnstr → PolyCnstr
   | .le p => .le p.norm
 
 def PolyCnstr.divAll (k : Int) : PolyCnstr → Bool
-  | .eq p => p.divAll k
-  | .le p => p.divAll k
+  | .eq p | .le p => p.divAll k
+
+def PolyCnstr.divCoeffs (k : Int) : PolyCnstr → Bool
+  | .eq p | .le p => p.divCoeffs k
+
+def PolyCnstr.isLe : PolyCnstr → Bool
+  | .eq _ => false
+  | .le _ => true
 
 def PolyCnstr.div (k : Int) : PolyCnstr → PolyCnstr
   | .eq p => .eq <| p.div k
@@ -130,6 +181,10 @@ inductive ExprCnstr  where
   | eq (p₁ p₂ : Expr)
   | le (p₁ p₂ : Expr)
   deriving Inhabited, BEq
+
+def ExprCnstr.isLe : ExprCnstr → Bool
+  | .eq .. => false
+  | .le .. => true
 
 def ExprCnstr.denote (ctx : Context) : ExprCnstr → Prop
   | .eq e₁ e₂ => e₁.denote ctx = e₂.denote ctx
@@ -177,7 +232,7 @@ attribute [local simp] Poly.div Poly.divAll PolyCnstr.denote
 
 theorem Poly.denote_div_eq_of_divAll (ctx : Context) (p : Poly) (k : Int) : p.divAll k → (p.div k).denote ctx * k = p.denote ctx := by
   induction p with
-  | num _ => simp
+  | num _ => simp; intro h; rw [← cdiv_eq_div_of_divides h]; assumption
   | add k' v p ih =>
     simp; intro h₁ h₂
     have ih := ih h₂
@@ -187,9 +242,9 @@ theorem Poly.denote_div_eq_of_divAll (ctx : Context) (p : Poly) (k : Int) : p.di
 
 attribute [local simp] Poly.divCoeffs Poly.getConst
 
-theorem Poly.denote_div_eq_of_divCoeffs (ctx : Context) (p : Poly) (k : Int) : p.divCoeffs k → (p.div k).denote ctx * k + p.getConst % k = p.denote ctx := by
+theorem Poly.denote_div_eq_of_divCoeffs (ctx : Context) (p : Poly) (k : Int) : p.divCoeffs k → (p.div k).denote ctx * k + cmod p.getConst k = p.denote ctx := by
   induction p with
-  | num k' => simp; rw [Int.add_comm, Int.mul_comm, Int.ediv_add_emod]
+  | num k' => simp; rw [Int.mul_comm, cdiv_add_cmod]
   | add k' v p ih =>
     simp; intro h₁ h₂
     rw [← ih h₂]
@@ -305,7 +360,7 @@ attribute [local simp] PolyCnstr.divAll PolyCnstr.div
 
 theorem ExprCnstr.eq_of_toPoly_eq_of_divBy' (ctx : Context) (e e' : ExprCnstr) (p : PolyCnstr) (k : Int) : k > 0 → p.divAll k → e.toPoly = p → e'.toPoly = p.div k → e.denote ctx = e'.denote ctx := by
   intro h₀ h₁ h₂ h₃
-  have hz : k ≠ 0 := by intro h; simp [h] at h₀
+  have hz : k ≠ 0 := Int.ne_of_gt h₀
   cases p <;> simp at h₁
   next p =>
     replace h₁ := Poly.denote_div_eq_of_divAll ctx p k h₁
@@ -329,11 +384,66 @@ theorem ExprCnstr.eq_of_toPoly_eq_of_divBy' (ctx : Context) (e e' : ExprCnstr) (
     rw [denote_toPoly, denote_toPoly] at this
     exact this
 
-theorem ExprCnstr.eq_of_toPoly_eq_of_divBy (ctx : Context) (e e' : ExprCnstr) (k : Int) : divBy e e' k → e.denote ctx = e'.denote ctx := by
+theorem ExprCnstr.eq_of_divBy (ctx : Context) (e e' : ExprCnstr) (k : Int) : divBy e e' k → e.denote ctx = e'.denote ctx := by
   intro h
   simp only [divBy, Bool.and_eq_true, bne_iff_ne, ne_eq, beq_iff_eq, decide_eq_true_eq] at h
   have ⟨⟨h₁, h₂⟩, h₃⟩ := h
   exact ExprCnstr.eq_of_toPoly_eq_of_divBy' ctx e e' e.toPoly k h₁ h₂ rfl h₃
+
+private theorem mul_add_cmod_le_iff {a k b : Int} (h : k > 0) : a*k + cmod b k ≤ 0 ↔ a ≤ 0 := by
+  constructor
+  · intro h'
+    have h₁ : a*k ≤ -cmod b k := by
+      have := Int.le_sub_right_of_add_le h'
+      simp at this
+      assumption
+    have h₂ : -cmod b k < k := by
+      have := cmod_gt_of_pos b h
+      have := Int.neg_lt_neg this
+      simp at this
+      assumption
+    have h₃ : a*k < k := Int.lt_of_le_of_lt h₁ h₂
+    have h₄ : a < 1 := by
+      conv at h₃ => rhs; rw [← Int.one_mul k]
+      have := Int.lt_of_mul_lt_mul_right h₃ (Int.le_of_lt h)
+      assumption
+    exact Int.le_of_lt_add_one (h₄ : a < 0 + 1)
+  · intro h'
+    have : a * k ≤ 0 := Int.mul_nonpos_of_nonpos_of_nonneg h' (Int.le_of_lt h)
+    have := Int.add_le_add this (cmod_nonpos b (Int.ne_of_gt h))
+    simp at this
+    assumption
+
+theorem ExprCnstr.eq_of_toPoly_eq_of_divCoeffs (ctx : Context) (e e' : ExprCnstr) (p : PolyCnstr) (k : Int) : k > 0 → p.divCoeffs k → p.isLe → e.toPoly = p → e'.toPoly = p.div k → e.denote ctx = e'.denote ctx := by
+  intro h₀ h₁ h₂ h₃ h₄
+  have hz : k ≠ 0 := Int.ne_of_gt h₀
+  cases p <;> simp [PolyCnstr.isLe] at h₂
+  clear h₂
+  next p =>
+    simp [PolyCnstr.divCoeffs] at h₁
+    replace h₁ := Poly.denote_div_eq_of_divCoeffs ctx p k h₁
+    replace h₃ := congrArg (PolyCnstr.denote ctx) h₃
+    simp only [PolyCnstr.denote.eq_2, ← h₁] at h₃
+    replace h₄ := congrArg (PolyCnstr.denote ctx) h₄
+    simp only [PolyCnstr.denote.eq_2, PolyCnstr.div] at h₄
+    rw [denote_toPoly] at h₃ h₄
+    rw [h₃, h₄]
+    apply propext
+    apply mul_add_cmod_le_iff
+    exact h₀
+
+-- Certificate for normalizing the coefficients of inequality constraint with bound tightening
+def divByLe (e e' : ExprCnstr) (k : Int) : Bool :=
+  k > 0 && e.isLe && e.toPoly.divCoeffs k && e'.toPoly == e.toPoly.div k
+
+theorem ExprCnstr.eq_of_divByLe (ctx : Context) (e e' : ExprCnstr) (k : Int) : divByLe e e' k → e.denote ctx = e'.denote ctx := by
+  intro h
+  simp only [divByLe, Bool.and_eq_true, bne_iff_ne, ne_eq, beq_iff_eq, decide_eq_true_eq] at h
+  have ⟨⟨⟨h₀, h₁⟩, h₂⟩, h₃⟩ := h
+  have hle : e.toPoly.isLe := by
+    cases e <;> simp [ExprCnstr.isLe] at h₁
+    simp [PolyCnstr.isLe]
+  apply ExprCnstr.eq_of_toPoly_eq_of_divCoeffs ctx e e' e.toPoly k h₀ h₂ hle rfl h₃
 
 def PolyCnstr.isUnsat : PolyCnstr → Bool
   | .eq (.num k) => k != 0
@@ -351,10 +461,10 @@ theorem ExprCnstr.eq_false_of_isUnsat (ctx : Context) (c : ExprCnstr) (h : c.toP
   assumption
 
 def PolyCnstr.isUnsatCoeff (k : Int) : PolyCnstr → Bool
-  | .eq p => p.divCoeffs k && k > 0 && p.getConst % k > 0
+  | .eq p => p.divCoeffs k && k > 0 && cmod p.getConst k < 0
   | .le _ => false
 
-private theorem contra {a b k : Int} (h₀ : 0 < k) (h₁ : 0 < b) (h₂ : b < k) (h₃ : a*k + b = 0) : False := by
+private theorem contra_old {a b k : Int} (h₀ : 0 < k) (h₁ : 0 < b) (h₂ : b < k) (h₃ : a*k + b = 0) : False := by
   have : b = -a*k := by
     rw [← Int.neg_eq_of_add_eq_zero h₃, Int.neg_mul]
   rw [this] at h₁ h₂
@@ -366,14 +476,29 @@ private theorem contra {a b k : Int} (h₀ : 0 < k) (h₁ : 0 < b) (h₂ : b < k
   have : (1 : Int) < 1 := Int.lt_of_le_of_lt low high
   contradiction
 
-private theorem PolyCnstr.eq_false (ctx : Context) (p : Poly) (k : Int) : p.divCoeffs k → k > 0 → p.getConst % k > 0 → (PolyCnstr.eq p).denote ctx = False := by
+private theorem contra {a b k : Int} (h₀ : 0 < k) (h₁ : -k < b) (h₂ : b < 0) (h₃ : a*k + b = 0) : False := by
+  have : b = -a*k := by
+    rw [← Int.neg_eq_of_add_eq_zero h₃, Int.neg_mul]
+  rw [this, Int.neg_mul] at h₁ h₂
+  replace h₁ := Int.lt_of_neg_lt_neg h₁
+  replace h₂ : -(a*k) < -0 := h₂
+  replace h₂ := Int.lt_of_neg_lt_neg h₂
+  replace h₁ : a * k < 1 * k := by simp [h₁]
+  replace h₁ : a < 1 := Int.lt_of_mul_lt_mul_right h₁ (Int.le_of_lt h₀)
+  replace h₂ : 0 * k < a * k := by simp [h₂]
+  replace h₂ : 0 < a := Int.lt_of_mul_lt_mul_right h₂ (Int.le_of_lt h₀)
+  replace h₂ : 1 ≤ a := h₂
+  have : (1 : Int) < 1 := Int.lt_of_le_of_lt h₂ h₁
+  contradiction
+
+private theorem PolyCnstr.eq_false (ctx : Context) (p : Poly) (k : Int) : p.divCoeffs k → k > 0 → cmod p.getConst k < 0 → (PolyCnstr.eq p).denote ctx = False := by
   simp
   intro h₁ h₂ h₃ h
   have hnz : k ≠ 0 := by intro h; rw [h] at h₂; contradiction
   have := Poly.denote_div_eq_of_divCoeffs ctx p k h₁
   rw [h] at this
-  have low := h₃
-  have high := Int.emod_lt_of_pos p.getConst h₂
+  have low := cmod_gt_of_pos p.getConst h₂
+  have high := h₃
   exact contra h₂ low high this
 
 theorem ExprCnstr.eq_false_of_isUnsat_coeff (ctx : Context) (c : ExprCnstr) (k : Int) : c.toPoly.isUnsatCoeff k → c.denote ctx = False := by
